\documentclass{article}
\usepackage{amsmath}

\begin{document}
\title{ASSIGNMENT 4}
\author{Showqeen Yousuf}
\date{\today}
\maketitle

\begin{itemize}

\item{\textbf{Exercise:2.19:}}\\

$

If,

 \[
 A'=
 \begin{pmatrix}
 -2 & 3\\
 1 & 2 
 \end{pmatrix}
 \] and
 $ 
  \[
 B=
 \begin{pmatrix}
 -1 & 0\\
 1 & 2 
 \end{pmatrix}
 \] then find $(A+2B)'$

 \item{\textbf{Solution:}}\\
 
 Given,\\
 \[
 A'=
 \begin{pmatrix}
 -2 & 3\\
 1 & 2 
 \end{pmatrix}
 \] and
 $\\
 
  \[
 B=
 \begin{pmatrix}
 -1 & 0\\
 1 & 2 
 \end{pmatrix}
 \]\\
 
 Now,\\
 
 \[
  A=(A')'=
 \begin{pmatrix}
 -2 & 1\\
 3 & 2 
 \end{pmatrix}
 \]
 and,   \[
 2B=
 \begin{pmatrix}
 -2 & 0\\
 2 & 4 
 \end{pmatrix}
 \]\\
 
 Now,\\
 
 \[
  A+2B=
 \begin{pmatrix}
 -2 & 1\\
 3 & 2 
 \end{pmatrix}
 +
 \begin{pmatrix}
 -2 & 0\\
 2 & 4 
 \end{pmatrix}
 \]\\
 
 Or, \[
  A+2B=
 \begin{pmatrix}
 -4 & 1\\
 5 & 6 
 \end{pmatrix}
 \] and\\
 
  \[
  (A+2B)'=
 \begin{pmatrix}
 -4 & 5\\
 1 & 6 
 \end{pmatrix}
 \]
 \\
 
 \item{\textbf{Exercise:2.21:}}\\

$

For the matrix,

 \[
 A=
 \begin{pmatrix}
 1 & 5\\
 6 & 7 
 \end{pmatrix}
 \]  verify that\\

\textbf{i)(A+A') is a symmetric matrix}.\\

\item{\textbf{Solution:}}\\
 
Given,\\
 \[
 A=
 \begin{pmatrix}
 1 & 5\\
 6 & 7 
 \end{pmatrix}
 \]\\
 
For matrix to be symmetric\\

$(A+A')=(A+A')'$\\
 
Now,\\
 \[
 A'=
 \begin{pmatrix}
 1 & 6\\
 5 & 7 
 \end{pmatrix}
 \]

 
 \[
 (A+A')=
 \begin{pmatrix}
 1 & 5\\
 6 & 7 
 \end{pmatrix}
 +
\begin{pmatrix}
 1 & 6\\
 5 & 7 
 \end{pmatrix}
 \] 
 
 Or,
 
 \[
 (A+A')=
 \begin{pmatrix}
 2 & 11\\
 11 & 14 
 \end{pmatrix}
 \] 

Also,\\

 \[
 (A+A')'=
 \begin{pmatrix}
 2 & 11\\
 11 & 14 
 \end{pmatrix}
 \] \\
 we get, $(A+A')=(A+A')'$\\
 
 Therefore, $(A+A')$ is symmetric.\\
 

\textbf{ii)(A-A') is a skew-symmetric matrix}.\\

\item{\textbf{Solution:}}\\
 
 Given,\\
 
 \[
 A=
 \begin{pmatrix}
 1 & 5\\
 6 & 7 
 \end{pmatrix}
 \]\\
 
For matrix to be skew-symmetric\\

$(A-A')=-(A-A')'$\\
 
  Now,\\
 \[
 A'=
 \begin{pmatrix}
 1 & 6\\
 5 & 7 
 \end{pmatrix}
 \]

 
 \[
 (A-A')=
 \begin{pmatrix}
 1 & 5\\
 6 & 7 
 \end{pmatrix}
 -
\begin{pmatrix}
 1 & 6\\
 5 & 7 
 \end{pmatrix}
 \] 
 
 Or,
 
 \[
 (A-A')=
 \begin{pmatrix}
 0 & -1\\
 1 & 0 
 \end{pmatrix}
 \] 

Also,\\

 \[
 (A-A')'=
 \begin{pmatrix}
 0 & 1\\
-1 & 0
 \end{pmatrix}
\]

and\\
\[
 -(A-A')'=
 \begin{pmatrix}
0 & -1\\
1 & 0
 \end{pmatrix}
 \]\\
 
 we get, $(A-A')=-(A-A')'$\\
 
 Therefore, $(A-A')$ is skew-symmetric.\\

\end{itemize}
\end{document}
